## ðŸ“˜ Square Root Tricks & Memorization

### ðŸ§  How to Know If a Number is a Perfect Square

#### âœ… Quick Tests:

- âœ” Ends in **0, 1, 4, 5, 6, 9** (âŒ Never ends in 2, 3, 7, 8)
- âœ” Digital Root âˆˆ {**1, 4, 7, 9**}  repetitive sum of digits 
- âœ” Prime factorization: All primes have **even powers**
- âœ” If ends in **25**, square root ends in **5**

---
#### ðŸŽ¯ Memorize from $0^2$ to $9^2$

```ts
//-------------------      Last Digit of Square
0*0 = 0^2 = 0                     0 
1*1 = 1^2 = 1                     1 -----------------
2*2 = 2^2 = 4                     4 --------------
3*3 = 3^2 = 9                     9 ------------
4*4 = 4^2 = 16                    6 --------
5*5 = 5^2 = 25                    5 ----
6*6 = 6^2 = 36                    6 --------
7*7 = 7^2 = 49                    9 ------------
8*8 = 8^2 = 64                    4 --------------
9*9 = 9^2 = 81                    1 -----------------
```

---

### ðŸ” Square Pattern Formula

 $(n + 1)^2 = n^2 + 2n + 1$

Use this to build squares mentally:
ðŸ§® Example:

172=289â‡’182=289+2Ã—17+1=289+34+1=32417^2 = 289 \Rightarrow 18^2 = 289 + 2Ã—17 + 1 = 289 + 34 + 1 = 324172=289â‡’182=289+2Ã—17+1=289+34+1=324

â« You can do the reverse too:

$(nâˆ’1)2=n2âˆ’2n+1(n - 1)^2 = n^2 - 2n + 1(nâˆ’1)2=n2âˆ’2n+1$

---

### ðŸŽ“ Tricks to Find âˆš(Perfect Square)

#### ðŸ“Œ 1. Check the **last digit**

- If a square ends in **9**, root ends in **3 or 7**
- If ends in **6**, root ends in **4 or 6**
- If ends in **5**, root must end in **5**
- If ends in **1**, root ends in **1 or 9**
- If ends in **4**, root ends in **2 or 8**

#### ðŸ“Œ 2. Use range estimation:

```csharp
Between n^2 and (n+1)^2 guess the root
```


```csharp
âˆš289 â†’ ends in 9 â†’ try 13 or 17 2 is before 89 â†’ try 17Â² = 289 âœ…
```

---

> [!quote]+ ðŸ§® Example
> If you know:
> $$
> 17^2 = 289
> $$
> Then use the identity:
> $$
> (n + 1)^2 = n^2 + 2n + 1
> $$
> Apply it:
> $$ > 18^2 = 289 + 2 \times 17 + 1 = 289 + 34 + 1 = 324 $$

---

> [!tip]+ â« You can do the reverse too:
>
> $$
> (n - 1)^2 = n^2 - 2n + 1
> $$
